update isabelle theories

isabelle/Hoare.thy
@@ -5,67 +5,63 @@ begin
 (* result of executing a loop body,
    runtime errors are represented as None *)
 datatype 'a res
-  = Ok 'a
-  | Break 'a
+  = Ok  'a
+  | Brk 'a
+  | Err
 
 (* TODO: get rid of option, to have working seq for both body and prog *)
 
 type_synonym 'a cond = "'a \<Rightarrow> bool"
 type_synonym 'a rel  = "'a \<Rightarrow> 'a \<Rightarrow> bool"
-type_synonym 'a body = "'a \<Rightarrow> ('a res) option \<Rightarrow> bool"
-type_synonym 'a prog = "'a \<Rightarrow> 'a option \<Rightarrow> bool"
-
-inductive breaks :: "'a body \<Rightarrow> bool" where
-breaksI[intro!]:
-  "c s (Some (Break s'))
-    \<Longrightarrow> breaks c"
+type_synonym 'a body = "'a \<Rightarrow> 'a res \<Rightarrow> bool"
+type_synonym 'a prog = "'a \<Rightarrow> 'a res \<Rightarrow> bool"
 
 (* Definition 1: Semantics of Loops *)
 inductive while :: "'a cond \<Rightarrow> 'a body \<Rightarrow> 'a prog" where
 while_baseI[intro]:
-  "\<lbrakk>\<not> t s\<rbrakk> \<Longrightarrow> while t B s (Some s)" |
+  "\<lbrakk>\<not> t s\<rbrakk> \<Longrightarrow> while t B s (Ok s)" |
 while_errI[intro]:
-  "\<lbrakk>t s; B s None\<rbrakk> \<Longrightarrow> while t B s None" |
+  "\<lbrakk>t s; B s Err\<rbrakk> \<Longrightarrow> while t B s Err" |
 while_breakI[intro]:
-  "\<lbrakk>t s; B s (Some (Break s'))\<rbrakk> \<Longrightarrow> while t B s (Some s')" |
+  "\<lbrakk>t s; B s (Brk s')\<rbrakk> \<Longrightarrow> while t B s (Ok s')" |
 while_stepI[intro]:
-  "\<lbrakk>t s; B s (Some (Ok s')); while t B s' s''\<rbrakk> \<Longrightarrow> while t B s s''"
+  "\<lbrakk>t s; B s (Ok s'); while t B s' s''\<rbrakk> \<Longrightarrow> while t B s s''"
 
 (* Definition 2: Validity of Hoare-Triples (partial correctness *)
 inductive hoare :: "'a cond \<Rightarrow> 'a prog \<Rightarrow> 'a cond \<Rightarrow> bool" where
 hoareI[intro!]:
-"\<lbrakk>\<And> s r. P s \<Longrightarrow> c s r \<Longrightarrow> \<exists> s'. r = Some s' \<and> Q s'\<rbrakk>
+"\<lbrakk>\<And> s r. P s \<Longrightarrow> c s r \<Longrightarrow> \<exists> s'. r = Ok s' \<and> Q s'\<rbrakk>
   \<Longrightarrow> hoare P c Q"
 
 lemma hoareE[elim]:
   assumes "hoare P c Q"
   assumes "P s" "c s r"
-  obtains s' where "r = Some s'" "Q s'"
+  obtains s' where "r = Ok s'" "Q s'"
   using assms by (blast elim: hoare.cases)
 
 (* Only safety of Hoare Triples *)
 
 inductive safe :: "'a cond \<Rightarrow> 'a prog \<Rightarrow> bool" where
 safeI[intro!]:
-"\<lbrakk>\<And> s r. P s \<Longrightarrow> c s r \<Longrightarrow> \<exists> s'. r = Some s'\<rbrakk>
+"\<lbrakk>\<And> s r. P s \<Longrightarrow> c s r \<Longrightarrow> \<exists> s'. r = Ok s'\<rbrakk>
   \<Longrightarrow> safe P c"
 
 lemma safeE[elim]:
   assumes "safe P c"
   assumes "P s" "c s r"
-  obtains s' where "r = Some s'"
+  obtains s' where "r = Ok s'"
   using assms by (blast elim: safe.cases)
 
 (* Weak variant of Hoare-Triples where runtime errors are not considered *)
 
 inductive correct :: "'a cond \<Rightarrow> 'a prog \<Rightarrow> 'a cond \<Rightarrow> bool" where
 correctI[intro!]:
-"\<lbrakk>\<And> s s'. P s \<Longrightarrow> c s (Some s' ) \<Longrightarrow> Q s'\<rbrakk>
+"\<lbrakk>\<And> s s'. P s \<Longrightarrow> c s (Ok s' ) \<Longrightarrow> Q s'\<rbrakk>
   \<Longrightarrow> correct P c Q"
 
 lemma correctE[elim]:
   assumes "correct P c Q"
-  assumes "P s" "c s (Some s' )"
+  assumes "P s" "c s (Ok s' )"
   shows "Q s'"
   using assms by (blast elim: correct.cases)
 
@@ -79,8 +75,8 @@ next
   show ?case proof (rule hoareI)
     fix s r
     assume c: "P s" "c s r"
-    from 2 c obtain s' where r: "r = Some s'" by blast (* need to make this explicit for Isabelle *)
-    from 2 c r show "\<exists>s'. r = Some s' \<and> Q s'"
+    from 2 c obtain s' where r: "r = Ok s'" by blast (* need to make this explicit for Isabelle *)
+    from 2 c r show "\<exists>s'. r = Ok s' \<and> Q s'"
       by auto
   qed
 qed
