isabelle/Summaries.thy
@@ -6,8 +6,8 @@ begin
 inductive summary_correct :: "'a cond \<Rightarrow> 'a cond \<Rightarrow> 'a body \<Rightarrow> 'a rel \<Rightarrow> 'a cond \<Rightarrow> bool" where
 summary_correctI[intro!]:
 "\<lbrakk>\<And> s.       \<lbrakk>\<not> t s\<rbrakk> \<Longrightarrow> R s s;
-  \<And> s s'.    \<lbrakk>t s; B s (Some (Break s'))\<rbrakk> \<Longrightarrow> R s s';
-  \<And> s s' sn. \<lbrakk>t s; R s' sn; B s (Some (Ok s'))\<rbrakk> \<Longrightarrow> R s sn;
+  \<And> s s'.    \<lbrakk>t s; B s (Brk s')\<rbrakk> \<Longrightarrow> R s s';
+  \<And> s s' sn. \<lbrakk>t s; R s' sn; B s (Ok s')\<rbrakk> \<Longrightarrow> R s sn;
   \<And> s0 sn.   \<lbrakk>P s0; R s0 sn\<rbrakk> \<Longrightarrow> Q sn\<rbrakk>
   \<Longrightarrow> summary_correct P t B R Q"
 
@@ -15,7 +15,7 @@ inductive_cases summary_correctE[elim!]: "summary_correct P t B R Q"
 
 lemma summary_post:
   assumes "while t B s r"
-  assumes "r = Some s'"
+  assumes "r = Ok s'"
   assumes "summary_correct P t B R Q"
   assumes "P s"
   shows   "Q s'"
@@ -37,13 +37,13 @@ inductive suffix :: "'a cond \<Rightarrow> 'a body \<Rightarrow> 'a rel" where
 suffix_baseI[intro]:
   "\<lbrakk>\<not> t s\<rbrakk> \<Longrightarrow> suffix t B s s" |
 suffix_breakI[intro]:
-  "\<lbrakk>t s; B s (Some (Break s'))\<rbrakk> \<Longrightarrow> suffix t B s s'" |
+  "\<lbrakk>t s; B s (Brk s')\<rbrakk> \<Longrightarrow> suffix t B s s'" |
 suffix_stepI[intro]:
-  "\<lbrakk>t s; B s (Some (Ok s')); suffix t B s' s''\<rbrakk> \<Longrightarrow> suffix t B s s''"
+  "\<lbrakk>t s; B s (Ok s'); suffix t B s' s''\<rbrakk> \<Longrightarrow> suffix t B s s''"
 
 lemma suffix_while[intro]:
   assumes "suffix t B s s'"
-  shows   "while t B s (Some s')"
+  shows   "while t B s (Ok s')"
   using assms by induction auto
 
 (* Theorem 4: Completeness of Loop Summaries wrt. Safe Invariants *)
@@ -55,5 +55,6 @@ proof -
     using assms by auto
   then show ?thesis ..
 qed
+
 
 end
